vera/SMT.v
@@ -1,81 +1,329 @@
 From Coq Require Import ZArith.
 From Coq Require Import BinNums.
 From Coq Require Import String.
+From Coq Require Import List.
+From Coq Require Import Logic.FunctionalExtensionality.
+From Coq Require Import Logic.ProofIrrelevance.
+Import ListNotations.
+
+From Equations Require Import Equations.
 
 From vera Require Import Common.
 From vera Require Import Bitvector.
+From vera Require VerilogSemantics.
+From vera Require Import Verilog.
+From vera Require Import Tactics.
+Import VerilogSemantics.CombinationalOnly.
+Import VerilogSMTBijection (bij_inverse, bij_apply, bij_wf).
+Import (coercions) VerilogSMTBijection.
+
+From SMTCoq Require Import bva.BVList.
+Import BITVECTOR_LIST.
 
 From SMTCoqApi Require SMTLib.
+From SMTCoqApi Require SMTLibFacts.
 
 Module SMT.
-  Inductive qfbv {T} :=
-  | BVOr : qfbv -> qfbv -> qfbv
-  | BVAnd : qfbv -> qfbv -> qfbv
-  | BVAdd : qfbv -> qfbv -> qfbv
-  | BVMul : qfbv -> qfbv -> qfbv
-  | BVNeg : qfbv -> qfbv
-  | BVNot : qfbv -> qfbv
-  | BVShl : qfbv -> qfbv -> qfbv
-  | BVLShr : qfbv -> qfbv -> qfbv
-  | BVLit : BV.t -> qfbv
-  | BVVar : T -> qfbv
-  | BVZeroExtend : N -> qfbv -> qfbv
-  | BVExtract : N -> N -> qfbv -> qfbv
-  | BVConcat : qfbv -> qfbv -> qfbv
-  | CoreEq : qfbv -> qfbv -> qfbv
-  | CoreNot : qfbv -> qfbv
-  | CoreITE : qfbv -> qfbv -> qfbv -> qfbv
-  .
+  Definition match_map_verilog (tag : TaggedName.Tag) (map : VerilogSMTBijection.t) verilog :=
+    forall verilogName,
+      (exists smtName, map (tag, verilogName) = Some smtName)
+      <-> (In verilogName (variable_names (Verilog.modVariables verilog))).
 
-  Arguments qfbv : clear implicits.
-
-  Inductive sort :=
-  | SBitVector : N -> sort
-  .
-
-  Inductive formula {T} :=
-  | CDeclare : T -> sort -> formula
-  | CEqual : qfbv T -> qfbv T -> formula
-  | CDistinct : qfbv T -> qfbv T -> formula
-  .
-
-  Arguments formula : clear implicits.
-
-  Record smt_netlist {name : Type} : Type :=
-    SMTNetlist
-      { smtnlName : string
-      ; smtnlPorts : list (name * port_direction)
-      ; smtnlFormulas : list (formula name)
+  Record smt_with_namemap :=
+    MkSMTWithNameMap
+      { query : SMTLib.query;
+        widths : list (nat * N);
+        nameMap : VerilogSMTBijection.t;
       }.
 
-  Arguments smt_netlist : clear implicits.
+  Remark match_map_verilog_width tag map verilog smtName verilogName :
+    match_map_verilog tag map verilog ->
+    map (tag, verilogName) = Some smtName ->
+    exists width, In (verilogName, width) (variable_widths (Verilog.modVariables verilog)).
+  Proof.
+    intros H1 H2.
+    apply variable_names_widths.
+    eapply H1.
+    eauto.
+  Qed.
 
-  Record smtlib_query :=
-    MkSMTLibQuery
-      { nameSMTToVerilog : NatFunMap.t string;
-        nameVerilogToSMT : StrFunMap.t (nat * SMTLib.sort);
-        declarations : list (nat * SMTLib.sort);
-        assertions : list SMTLib.term
-      }.
+  Definition max_var (q : SMTLib.query) : nat :=
+    List.list_max (SMTLibFacts.domain q).
 
-  Definition model interp_sort_sym :=
-    forall (n : nat) (dom : list SMTLib.sort) (codom : SMTLib.sort), SMTLib.interp_fun_type interp_sort_sym dom codom.
+  Program Definition valuation_of_execution (m : VerilogSMTBijection.t) (e : execution) : SMTLib.valuation :=
+    fun n =>
+    match bij_inverse m n with
+    | None => None
+    | Some (_, vname) =>
+        match e vname with
+        | None => None
+        | Some xbv =>
+            match XBV.to_bv xbv with
+            (* TODO: Fix handling of Xs *)
+            | None => None
+            | Some val => Some (SMTLib.Value_BitVec (N.of_nat (length val)) {| bv := val |})
+            end
+        end
+    end.
 
-  Definition no_uninterp_sorts : nat -> Type := fun _ => False.
+  Definition execution_of_valuation (tag : TaggedName.Tag) (m : VerilogSMTBijection.t) (v : SMTLib.valuation) : execution :=
+      fun vname =>
+        match m (tag, vname) with
+        | Some smtName =>
+            match v smtName with
+            | Some (SMTLib.Value_BitVec _ bv) => Some (XBV.from_bv bv)
+            | _ => None
+            end
+        | None => None
+        end
+    .
 
-  Definition max_var (q : smtlib_query) : nat :=
-    List.list_max (List.map fst (declarations q)).
+  Lemma execution_of_valuation_some tag (m : VerilogSMTBijection.t) ρ smtName vname sz bv :
+    m (tag, vname) = Some smtName ->
+    ρ smtName = Some (SMTLib.Value_BitVec sz bv) ->
+    execution_of_valuation tag m ρ vname = Some (XBV.from_bv bv).
+  Proof.
+    unfold execution_of_valuation.
+    intros H1 H2.
+    now (rewrite H1; rewrite H2).
+  Qed.
 
-  Definition satisfied_by
-    (query : smtlib_query)
-    (interp_sort_sym : nat -> Type)
-    (interp_fun_sym : model interp_sort_sym) :=
-    List.Forall
-      (fun term => SMTLib.interp_term interp_sort_sym interp_fun_sym term =
-                  Some (existT _ SMTLib.Sort_Bool true))
-      (assertions query).
+  Program Definition valuation_of_executions (m : VerilogSMTBijection.t) (e1 e2 : execution) : SMTLib.valuation :=
+    fun n =>
+    match bij_inverse m n with
+    | None => None
+    | Some (t, vname) =>
+        let e :=
+          match t with
+          | TaggedName.VerilogLeft => e1
+          | TaggedName.VerilogRight => e2
+          end
+        in
+        match e vname with
+        | None => None
+        | Some xbv =>
+            match XBV.to_bv xbv with
+            (* TODO: Fix handling of Xs *)
+            | None => None
+            | Some val => Some (SMTLib.Value_BitVec (N.of_nat (length val)) {| bv := val |})
+            end
+        end
+    end.
 
-  Definition sat (query : smtlib_query) : Prop := exists interp_sort_sym interp_fun_sym, satisfied_by query interp_sort_sym interp_fun_sym.
+  Lemma execution_left_of_valuation_of_executions m v e1 e2 :
+    (* TODO: Remove assumption *)
+    (forall n xbv, e1 n = Some xbv -> ~ XBV.has_x xbv) ->
+    (forall n xbv, e2 n = Some xbv -> ~ XBV.has_x xbv) ->
+    match_map_verilog TaggedName.VerilogLeft m v ->
+    complete_execution v e1 ->
+    execution_of_valuation TaggedName.VerilogLeft m (valuation_of_executions m e1 e2) = e1.
+  Proof.
+    intros * Hno_exes1 Hno_exes2 Hmatch Hcomplete.
+    unfold valuation_of_executions.
+    unfold execution_of_valuation.
+    apply functional_extensionality.
+    intros name.
+    autodestruct_eqn E; simpl in *; try subst.
+    - replace s with name in * by
+        (apply bij_wf in E; congruence).
+      rewrite E3. f_equal.
+      apply XBV.bv_xbv_inverse. assumption.
+    - apply bij_wf in E.
+      congruence.
+    - replace s with name in * by
+          (apply bij_wf in E; congruence).
+      apply Hno_exes1 in E3.
+      rewrite <- XBV.has_x_to_bv in E4.
+      contradiction.
+    - replace s with name in * by
+          (apply bij_wf in E; congruence).
+      apply Hno_exes2 in E3.
+      rewrite <- XBV.has_x_to_bv in E4.
+      contradiction.
+    - replace s with name in * by
+         (apply bij_wf in E; congruence).
+      auto.
+    - apply bij_wf in E; congruence.
+    - apply bij_wf in E; congruence.
+    - destruct (e1 name) as [xbv |] eqn:E1; try reflexivity.
+      enough (exists xbv', m (TaggedName.VerilogLeft, name) = Some xbv')
+        as [? ?] by congruence.
+      destruct (Hmatch name) as [_ H].
+      edestruct H as [smtName HsmtName]. {
+        unfold complete_execution in Hcomplete.
+        apply Hcomplete. exists xbv. auto.
+      }
+      eauto.
+  Qed.
 
-  Definition unsat (query : smtlib_query) : Prop := forall interp_sort_sym interp_fun_sym, ~ (satisfied_by query interp_sort_sym interp_fun_sym).
+  Lemma execution_right_of_valuation_of_executions m v e1 e2 :
+    (* TODO: Remove assumption *)
+    (forall n xbv, e1 n = Some xbv -> ~ XBV.has_x xbv) ->
+    (forall n xbv, e2 n = Some xbv -> ~ XBV.has_x xbv) ->
+    match_map_verilog TaggedName.VerilogRight m v ->
+    complete_execution v e2 ->
+    execution_of_valuation TaggedName.VerilogRight m (valuation_of_executions m e1 e2) = e2.
+  Proof.
+    intros * Hno_exes1 Hno_exes2 Hmatch Hcomplete.
+    unfold valuation_of_executions.
+    unfold execution_of_valuation.
+    apply functional_extensionality.
+    intros name.
+    autodestruct_eqn E; simpl in *; try subst.
+    - apply bij_wf in E.
+      congruence.
+    - replace s with name in * by
+        (apply bij_wf in E; congruence).
+      rewrite E3. f_equal.
+      apply XBV.bv_xbv_inverse. assumption.
+    - replace s with name in * by
+          (apply bij_wf in E; congruence).
+      apply Hno_exes1 in E3.
+      rewrite <- XBV.has_x_to_bv in E4.
+      contradiction.
+    - replace s with name in * by
+          (apply bij_wf in E; congruence).
+      apply Hno_exes2 in E3.
+      rewrite <- XBV.has_x_to_bv in E4.
+      contradiction.
+    - apply bij_wf in E; congruence.
+    - replace s with name in * by
+         (apply bij_wf in E; congruence).
+      auto.
+    - apply bij_wf in E; congruence.
+    - destruct (e2 name) as [xbv |] eqn:E1; try reflexivity.
+      enough (exists xbv', m (TaggedName.VerilogRight, name) = Some xbv')
+        as [? ?] by congruence.
+      destruct (Hmatch name) as [_ H].
+      edestruct H as [smtName HsmtName]. {
+        unfold complete_execution in Hcomplete.
+        apply Hcomplete. exists xbv. auto.
+      }
+      eauto.
+  Qed.
+
+  Lemma valuation_of_executions_some_left nameVerilog nameSMT xbv bv (m : VerilogSMTBijection.t) e1 e2 :
+    e1 nameVerilog = Some xbv ->
+    XBV.to_bv xbv = Some bv ->
+    m (TaggedName.VerilogLeft, nameVerilog) = Some nameSMT ->
+    (valuation_of_executions m e1 e2) nameSMT =
+      Some (SMTLib.Value_BitVec (BV.size bv) (of_bits bv)).
+  Proof.
+    intros Hexec Hexes Hname.
+    unfold valuation_of_executions; simpl.
+
+    pose proof (bij_wf m) as Hinverse.
+    specialize (Hinverse (TaggedName.VerilogLeft, nameVerilog) nameSMT).
+    apply Hinverse in Hname. clear Hinverse.
+    rewrite Hname.
+
+    rewrite Hexec.
+    rewrite Hexes.
+    repeat f_equal.
+
+    unfold of_bits.
+
+    f_equal.
+    apply proof_irrelevance.
+  Qed.
+
+  Lemma valuation_of_executions_some_right nameVerilog nameSMT xbv bv (m : VerilogSMTBijection.t) e1 e2 :
+    e2 nameVerilog = Some xbv ->
+    XBV.to_bv xbv = Some bv ->
+    m (TaggedName.VerilogRight, nameVerilog) = Some nameSMT ->
+    (valuation_of_executions m e1 e2) nameSMT =
+      Some (SMTLib.Value_BitVec (BV.size bv) (of_bits bv)).
+  Proof.
+    intros Hexec Hexes Hname.
+    unfold valuation_of_executions; simpl.
+
+    pose proof (bij_wf m) as Hinverse.
+    specialize (Hinverse (TaggedName.VerilogRight, nameVerilog) nameSMT).
+    apply Hinverse in Hname. clear Hinverse.
+    rewrite Hname.
+
+    rewrite Hexec.
+    rewrite Hexes.
+    repeat f_equal.
+
+    unfold of_bits.
+
+    f_equal.
+    apply proof_irrelevance.
+  Qed.
+
+  Section inverse.
+    Variable m : VerilogSMTBijection.t.
+    Variable v : Verilog.vmodule.
+    Variable e : execution.
+    Variable tag : TaggedName.Tag.
+    Context (Hcomplete : complete_execution v e).
+    Context (Hmatch : match_map_verilog tag m v).
+
+    Lemma valuation_of_execution_some nameVerilog nameSMT xbv bv :
+      e nameVerilog = Some xbv ->
+      XBV.to_bv xbv = Some bv ->
+      m (tag, nameVerilog) = Some nameSMT ->
+      (valuation_of_execution m e) nameSMT =
+        Some (SMTLib.Value_BitVec (BV.size bv) (of_bits bv)).
+    Proof.
+      intros Hexec Hexes Hname.
+      unfold valuation_of_execution; simpl.
+
+      pose proof (bij_wf m) as Hinverse.
+      specialize (Hinverse (tag, nameVerilog) nameSMT).
+      apply Hinverse in Hname.
+      rewrite Hname.
+
+      rewrite Hexec.
+      rewrite Hexes.
+      repeat f_equal.
+
+      unfold of_bits.
+
+      f_equal.
+      apply proof_irrelevance.
+    Qed.
+
+    Lemma execution_of_valuation_of_execution :
+      (* TODO: Remove assumption *)
+      (forall n xbv, e n = Some xbv -> ~ XBV.has_x xbv) -> 
+      execution_of_valuation tag m (valuation_of_execution m e) = e.
+    Proof.
+      intros Hno_exes.
+      apply functional_extensionality. intros verilogName.
+      unfold execution_of_valuation.
+      destruct (m (tag, verilogName)) as [name | ] eqn:Hname; try discriminate.
+      - unfold complete_execution in *. 
+        unfold match_map_verilog in Hmatch.
+        specialize (Hcomplete verilogName). simpl in *.
+        destruct Hcomplete as [Hcomplete' _]; clear Hcomplete.
+        edestruct Hcomplete' as [xbv Hxbv_val]. { firstorder. }
+        clear Hcomplete'.
+
+        unfold valuation_of_execution.
+
+        pose proof (bij_wf m) as Hinverse.
+        specialize (Hinverse (tag, verilogName) name).
+        apply Hinverse in Hname.
+        rewrite Hname.
+
+        rewrite Hxbv_val.
+
+        specialize (Hno_exes verilogName xbv ltac:(assumption)).
+        apply XBV.not_has_x_to_bv in Hno_exes.
+        destruct Hno_exes as [bv Hno_exes].
+        rewrite Hno_exes.
+        now erewrite XBV.bv_xbv_inverse.
+      - destruct (e verilogName) as [xbv |] eqn:E; try reflexivity.
+        enough (exists xbv', m (tag, verilogName) = Some xbv')
+          as [? ?] by congruence.
+        destruct (Hmatch verilogName) as [_ H].
+        edestruct H as [smtName HsmtName]. {
+          unfold complete_execution in Hcomplete.
+          apply Hcomplete. exists xbv. auto.
+        }
+        eauto.
+    Qed.
+  End inverse.
 End SMT.
