vera/VerilogEquivalence.v
@@ -1,9 +1,13 @@
 From vera Require Import Verilog.
 From vera Require Import SMT.
+Import (coercions) SMT.
 From vera Require Import Common.
+Import (coercions) VerilogSMTBijection.
+Import VerilogSMTBijection (bij_inverse, bij_apply, bij_wf).
 From vera Require VerilogTypecheck.
 From vera Require VerilogCanonicalize.
 From vera Require VerilogToSMT.
+From vera Require Import Decidable.
 
 From ExtLib Require Import Data.List.
 From ExtLib Require Import Data.Monads.EitherMonad.
@@ -22,6 +26,7 @@ From Coq Require Import ZArith.
 From Coq Require Import String.
 From Coq Require Import List.
 From Coq Require Import Sorting.Permutation.
+From Coq Require Import Structures.Equalities.
 
 Import ListNotations.
 Import CommonNotations.
@@ -30,94 +35,86 @@ Import FunctorNotation.
 Local Open Scope monad_scope.
 Local Open Scope string.
 
-Definition mk_equivalence_formulas
-  (inputs outputs : list string)
-  (namemap1 namemap2 : StrFunMap.t (nat * SMTLib.sort))
-  : sum string (list SMTLib.term) :=
-  inputs_same <-
-    mapT (fun n =>
-            match namemap1 n, namemap2 n with
-            | Some (smt_name1, SMTLib.Sort_BitVec size1),
-              Some (smt_name2, SMTLib.Sort_BitVec size2) =>
-                if (size1 =? size2)%N
-                then inr (SMTLib.Term_Eq
-                            (SMTLib.Term_Fun (smt_name1, ([], SMTLib.Sort_BitVec size1)) [])
-                            (SMTLib.Term_Fun (smt_name2, ([], SMTLib.Sort_BitVec size2)) []))
-                else inl "err"%string
-            | _, _ => inl "err"%string
-            end) inputs;;
+Equations mk_var_same (name : string) (namemap : VerilogSMTBijection.t)
+  : sum string SMTLib.term := {
+  | name, namemap with namemap (TaggedName.VerilogLeft, name), namemap (TaggedName.VerilogRight, name) => {
+    | Some smt_name1, Some smt_name2 =>
+        inr (SMTLib.Term_Eq (SMTLib.Term_Const smt_name1) (SMTLib.Term_Const smt_name2))
+    | _, _ => inl "mk_var_same"%string
+    }
+  }
+  .
 
-  outputs_different <-
-    mapT (
-        fun n =>
-          match namemap1 n, namemap2 n return sum string SMTLib.term with
-          | Some (smt_name1, SMTLib.Sort_BitVec size1),
-            Some (smt_name2, SMTLib.Sort_BitVec size2) =>
-              if (size1 =? size2)%N
-              then inr (SMTLib.Term_Not (SMTLib.Term_Eq
-                                           (SMTLib.Term_Fun (smt_name1, ([], SMTLib.Sort_BitVec size1)) [])
-                                           (SMTLib.Term_Fun (smt_name2, ([], SMTLib.Sort_BitVec size2)) [])))
-              else inl "err"%string
-          | _, _ => inl "err"%string
-          end) outputs;;
+Equations mk_inputs_same (inputs : list string) (namemap : VerilogSMTBijection.t)
+  : sum string SMTLib.term := {
+  | [], m => inr SMTLib.Term_True
+  | (name :: names), m =>
+      match
+        mk_var_same name m,
+        mk_inputs_same names m
+      with
+      | inr hd, inr tl =>
+          inr (SMTLib.Term_And hd tl)
+      | _, _ => inl "err"%string
+      end
+  }.
 
-  let outputs_different_any :=
-    List.fold_left
-      (fun acc q => SMTLib.Term_Or acc q)
-      outputs_different
-      SMTLib.Term_False
-  in
-  ret (app inputs_same [outputs_different_any])
-.
+Equations mk_var_distinct (name : string) (namemap : VerilogSMTBijection.t)
+  : sum string SMTLib.term := {
+  | name, namemap with namemap (TaggedName.VerilogLeft, name), namemap (TaggedName.VerilogRight, name) => {
+    | Some smt_name1, Some smt_name2 =>
+        inr (SMTLib.Term_Not (SMTLib.Term_Eq (SMTLib.Term_Const smt_name1) (SMTLib.Term_Const smt_name2)))
+    | _, _ => inl "mk_var_distinct"%string
+    }
+  }
+  .
 
-Axiom dec_permutation : forall (l1 l2 : list string), { Permutation l1 l2 } + { ~ Permutation l1 l2 }.
+Equations mk_outputs_distinct (inputs : list string) (namemap : VerilogSMTBijection.t)
+  : sum string SMTLib.term := {
+  | [], m => inr SMTLib.Term_False
+  | (name :: names), m =>
+      match
+        mk_var_distinct name m,
+        mk_outputs_distinct names m
+      with
+      | inr hd, inr tl =>
+          inr (SMTLib.Term_Or hd tl)
+      | _, _ => inl "err"%string
+      end
+  }.
 
-Definition assert_dec {P E} (dec : { P } + { ~ P }) (err : E) : sum E P :=
-  match dec with
-  | left prf => inr prf
-  | right _  => inl err
-  end
-.
-
-Definition equivalence_query_canonical
+Program Definition equivalence_query_canonical
   (canonical_verilog1 canonical_verilog2 : Verilog.vmodule)
-  : sum string (SMT.smtlib_query) :=
+  : sum string (SMT.smt_with_namemap) :=
 
   inputs_ok1 <- assert_dec
-                 (list_eq_dec string_dec (Verilog.inputs canonical_verilog1) (Verilog.inputs canonical_verilog2))
+                 ((Verilog.inputs canonical_verilog1) = (Verilog.inputs canonical_verilog2))
                  "Inputs don't match" ;;
 
   outputs_ok2 <- assert_dec
-                 (list_eq_dec string_dec (Verilog.outputs canonical_verilog1) (Verilog.outputs canonical_verilog2))
+                 ((Verilog.outputs canonical_verilog1) = (Verilog.outputs canonical_verilog2))
                  "Outputs don't match" ;;
 
-  query1 <- VerilogToSMT.verilog_to_smt 0 canonical_verilog1 ;;
-  query2 <- VerilogToSMT.verilog_to_smt (1 + SMT.max_var query1) canonical_verilog2 ;;
-  equivalence_formulas <-
-    mk_equivalence_formulas
-      (Verilog.inputs canonical_verilog1) (Verilog.outputs canonical_verilog1)
-      (SMT.nameVerilogToSMT query1) (SMT.nameVerilogToSMT query2) ;;
+  smt1 <- VerilogToSMT.verilog_to_smt TaggedName.VerilogLeft 0 canonical_verilog1 ;;
+  smt2 <- VerilogToSMT.verilog_to_smt TaggedName.VerilogRight (1 + SMT.max_var (SMT.query smt1)) canonical_verilog2 ;;
+
+  let nameMap := VerilogSMTBijection.combine (SMT.nameMap smt1) (SMT.nameMap smt2) _ _ in
+
+  inputs_same <- mk_inputs_same (Verilog.inputs canonical_verilog1) nameMap ;;
+  outputs_distinct <- mk_outputs_distinct (Verilog.outputs canonical_verilog1) nameMap ;;
 
   ret {|
-      SMT.nameSMTToVerilog :=
-        NatFunMap.combine
-          (NatFunMap.map (fun s => "left__" ++ s) (SMT.nameSMTToVerilog query1))
-          (NatFunMap.map (fun s => "right__" ++ s) (SMT.nameSMTToVerilog query2));
-      SMT.nameVerilogToSMT :=
-        StrFunMap.combine
-          (SMT.nameVerilogToSMT query1)
-          (SMT.nameVerilogToSMT query2);
-      SMT.declarations := SMT.declarations query1 ++ SMT.declarations query2;
-      SMT.assertions := SMT.assertions query1 ++ SMT.assertions query2 ++ equivalence_formulas
+      SMT.nameMap := nameMap ;
+      SMT.widths := SMT.widths smt1 ++ SMT.widths smt2;
+      SMT.query := (SMT.query smt1 ++ SMT.query smt2 ++ [inputs_same] ++ [outputs_distinct])%list
     |}
 .
+Next Obligation. (* No shared verilog names *) Admitted.
+Next Obligation. (* No shared SMT names *) Admitted.
 
-Definition equivalence_query (verilog1 verilog2 : Verilog.vmodule) : sum string SMT.smtlib_query :=
+Definition equivalence_query (verilog1 verilog2 : Verilog.vmodule) : sum string SMT.smt_with_namemap :=
   VerilogTypecheck.tc_vmodule verilog1 ;;
   VerilogTypecheck.tc_vmodule verilog2 ;;
-
-  inputs_ok1 <- assert_dec (list_eq_dec string_dec (Verilog.inputs verilog1) (Verilog.inputs verilog2)) "Inputs don't match" ;;
-  outputs_ok2 <- assert_dec (list_eq_dec string_dec (Verilog.outputs verilog1) (Verilog.outputs verilog2)) "Outputs don't match" ;;
 
   canonical_verilog1 <- VerilogCanonicalize.canonicalize_verilog verilog1 ;;
   canonical_verilog2 <- VerilogCanonicalize.canonicalize_verilog verilog2 ;;
