vera/VerilogEquivalenceCorrectness.v
@@ -1,6 +1,8 @@
 From vera Require Import Verilog.
 From vera Require Import SMT.
+Import (coercions) SMT.
 From vera Require Import Common.
+Import (coercions) VerilogSMTBijection.
 From vera Require Import Bitvector.
 From vera Require VerilogTypecheck.
 From vera Require VerilogCanonicalize.
@@ -8,11 +10,13 @@ From vera Require VerilogToSMT.
 From vera Require Import VerilogEquivalence.
 From vera Require VerilogSemantics.
 From vera Require Import Tactics.
+From vera Require Import Decidable.
 
 Import VerilogSemantics.CombinationalOnly.
 
 From Coq Require Import Relations.
 From Coq Require Import Sorting.Permutation.
+From Coq Require Import Lia.
 
 From Equations Require Import Equations.
 From ExtLib Require Import Structures.Monads.
@@ -34,21 +38,25 @@ Local Open Scope Z_scope.
 
 Definition match_on_regs
   (regs : list string)
-  (v1 v2 : VerilogState)
+  (st1 st2 : RegisterState)
   : Prop :=
   List.Forall
     (fun 'n =>
-       exists v, regState v1 n = Some v
-            /\ regState v2 n = Some v
+       exists v, st1 n = Some v
+            /\ st2 n = Some v
             /\ ~ XBV.has_x v
     ) regs.
 
-Definition no_errors (v : Verilog.vmodule) :=
-  forall (input_vals : list XBV.t)
-    (input_len_ok : length input_vals = length (Verilog.inputs v))
-    (input_vals_defined : Forall (fun bv => ~ XBV.has_x bv) input_vals),
-    let init := set_regs (List.combine (Verilog.inputs v) input_vals) (initial_state v) in
-    exists final, multistep_eval init final.
+Definition equivalent_behaviour v1 v2 :=
+  forall (input : list XBV.t)
+    (input_wf1 : input_valid v1 input)
+    (input_wf2 : input_valid v2 input)
+    (* (outputs_same : Verilog.outputs v1 = Verilog.outputs v2) *)
+    (input_vals_defined : Forall (fun bv => ~ XBV.has_x bv) input)
+    (final1 final2 : VerilogState),
+    run_multistep (initial_state v1 input) = Some final1 ->
+    run_multistep (initial_state v2 input) = Some final2 ->
+    match_on_regs (Verilog.outputs v1) (regState final1) (regState final2).
 
 Record equivalent (v1 v2 : Verilog.vmodule) : Prop :=
   MkEquivalent {
@@ -56,16 +64,7 @@ Record equivalent (v1 v2 : Verilog.vmodule) : Prop :=
       interface_outputs_match : Verilog.outputs v1 = Verilog.outputs v2;
       no_errors1 : no_errors v1;
       no_errors2 : no_errors v2;
-      behaviour_match :
-      forall (input_vals : list XBV.t)
-        (input_len_ok : length input_vals = length (Verilog.inputs v1))
-        (input_vals_defined : Forall (fun bv => ~ XBV.has_x bv) input_vals)
-        (final1 final2 : VerilogState),
-        let init1 := set_regs (List.combine (Verilog.inputs v1) input_vals) (initial_state v1) in
-        let init2 := set_regs (List.combine (Verilog.inputs v1) input_vals) (initial_state v2) in
-        multistep_eval init1 final1 ->
-        multistep_eval init2 final2 ->
-        match_on_regs (Verilog.outputs v1) final1 final2;
+      behaviour_match : equivalent_behaviour v1 v2;
     }
 .
 
@@ -104,143 +103,34 @@ Section V.
         AlwaysComb (BlockingAssign (NamedExpression 1%N "v") (NamedExpression 1%N "in"))
       ];
     |}.
+
+  Example assign_out_equivalent : equivalent assign_out assign_out.
+  Proof.
+    constructor; try auto.
+    - unfold no_errors. intros.
+      repeat (destruct input; try solve [simpl in *; discriminate]).
+      eexists.
+      repeat (unfold assign_out, set_reg, initial_state; simpl).
+      repeat (try econstructor; try unfold step; simpl; try simp run_step run_multistep exec_module_item exec_statement).
+    - unfold no_errors. intros.
+      repeat (destruct input; try solve [simpl in *; discriminate]).
+      eexists.
+      repeat (unfold assign_out, set_reg, initial_state; simpl).
+      repeat (try econstructor; try unfold step; simpl; try simp run_step run_multistep exec_module_item exec_statement).
+    - unfold equivalent_behaviour.
+      intros ? ? ? ? ? ? eval1 eval2.
+      repeat (destruct input; try solve [simpl in *; discriminate]).
+      unfold assign_out, set_reg in eval1; simpl in eval1.
+      unfold assign_out, set_reg in eval2; simpl in eval2.
+      repeat constructor.
+      repeat (simp run_multistep run_step exec_module_item exec_statement eval_expr in *; simpl in * );
+        unfold set_reg in *; simpl in *; try solve_by_inverts 3%nat.
+      inv eval1.
+      inv eval2.
+      eexists. intuition.
+      inv input_vals_defined. contradiction.
+  Qed.
 End V.
-
-Example assign_out_equivalent : equivalent assign_out assign_out.
-Proof.
-  constructor; try auto.
-  - unfold no_errors. intros.
-    repeat (destruct input_vals; try solve [simpl in *; discriminate]).
-    eexists.
-    repeat (unfold no_errors, assign_out, set_reg, initial_state; simpl).
-    repeat (try econstructor; try unfold step; simpl; try simp run_step exec_module_item exec_statement).
-  - unfold no_errors. intros.
-    repeat (destruct input_vals; try solve [simpl in *; discriminate]).
-    repeat (unfold no_errors, assign_out, set_reg, initial_state; simpl).
-    eexists.
-    repeat (try econstructor; try unfold step; simpl; try simp run_step exec_module_item exec_statement).
-  - unfold match_on_regs.
-    intros * ? ? * [eval1 blocked1] [eval2 blocked2].
-    simpl in input_len_ok.
-    repeat (destruct input_vals; try solve [simpl in *; discriminate]).
-    repeat (destruct input_vals_defined; try solve [simpl in *; discriminate]).
-    simpl in *.
-    unfold assign_out, set_reg in eval1; simpl in eval1.
-    unfold assign_out, set_reg in eval2; simpl in eval2.
-    repeat constructor.
-    unfold multistep_eval, multistep in *.
-    eapply clos_trans_t1n in eval1; inversion eval1 as [ ? step1 | ? ? step1_1 step1_2 ]; subst;
-      repeat (unfold step in *; simp run_step exec_module_item exec_statement eval_expr in *; simpl in * );
-      unfold set_reg in *; simpl in *; try solve_by_inverts 3%nat.
-    eapply clos_trans_t1n in eval2.
-    inversion eval2 as [ ? step2 | ? ? step2_1 step2_2 ]; subst;
-      repeat (unfold step in *; simp run_step exec_module_item exec_statement eval_expr in *; simpl in * );
-      unfold set_reg in *; simpl in *; try solve_by_inverts 3%nat.
-    inv step1.
-    inv step2.
-    eexists. intuition.
-Qed.
-
-Theorem canonicalize_correct v v' :
-  VerilogCanonicalize.canonicalize_verilog v = inr v' ->
-  equivalent v v'.
-Admitted.
-
-Definition match_on_regs_smt
-  (regs : list string)
-  (nameMap : StrFunMap.t (nat * SMTLib.sort))
-  (v : VerilogState)
-  (m : SMT.model SMT.no_uninterp_sorts)
-  : Prop :=
-  List.Forall
-    (fun regName =>
-       exists (varName : nat) (bv : BV.t),
-         regState v regName = Some (XBV.from_bv bv) /\
-           nameMap regName = Some (varName, SMTLib.Sort_BitVec (BV.size bv)) /\
-           m varName [] (SMTLib.Sort_BitVec (BV.size bv)) = BVList.BITVECTOR_LIST.of_bits bv
-    ) regs.
-
-Definition match_verilog_model
-  (nameMap : StrFunMap.t (nat * SMTLib.sort))
-  (v : Verilog.vmodule)
-  (m : SMT.model SMT.no_uninterp_sorts)
-  : Prop :=
-  forall (input_vals : list XBV.t)
-    (input_len_ok : length input_vals = length (Verilog.inputs v))
-    (input_vals_defined : Forall (fun bv => ~ XBV.has_x bv) input_vals)
-    (final : VerilogState),
-    let init := set_regs (List.combine (Verilog.inputs v) input_vals) (initial_state v) in
-    multistep_eval init final ->
-    match_on_regs_smt (Verilog.inputs v) nameMap init m ->
-    match_on_regs_smt (Verilog.outputs v) nameMap final m
-.
-
-Theorem verilog_to_smt_correct start v q :
-  VerilogToSMT.verilog_to_smt start v = inr q ->
-  forall model,
-  SMT.satisfied_by q (fun _ => False) model ->
-  match_verilog_model (SMT.nameVerilogToSMT q) v model.
-Admitted.
-
-Lemma mapT_list_sum_in {A B E} (f : A -> sum E B) (l : list A) (l' : list B) :
-  List.mapT_list f l = inr l' ->
-  forall x, In x l -> exists y, f x = inr y /\ In y l'.
-Proof.
-  generalize dependent f. generalize dependent l'.
-  induction l; intros * H * Hin; simpl in *.
-  - contradiction.
-  - destruct (f a) eqn:Hfa; try discriminate.
-    destruct (mapT_list f l) as [|tl] eqn:Heq; try discriminate.
-Admitted.
-
-Theorem equivalence_query_canonical_correct verilog1 verilog2 query :
-  equivalence_query_canonical verilog1 verilog2 = inr query ->
-  SMT.unsat query ->
-  equivalent verilog1 verilog2.
-Proof.
-  intros Hquery Hunsat.
-  unfold equivalence_query_canonical in *.
-  inv Hquery.
-  unfold mk_equivalence_formulas in *.
-  repeat (
-      match goal with
-      | [ H : (match ?m with _ => _ end) = _ |- _ ] =>
-          destruct m eqn:?; try discriminate
-      | [ H : inr _ = inr _ |- _ ] => inv H
-      | [ H : assert_dec _ _ = inr _ |- _ ] => clear H
-      | [ H : VerilogToSMT.verilog_to_smt _ _ = inr _ |- _ ] =>
-          pose proof (verilog_to_smt_correct _ _ _ H); clear H
-      | [ H : mapT_list _ _ = inr _ |- _ ] =>
-          learn (mapT_list_sum_in _ _ _ H)
-      end; simpl in *
-    ).
-  repeat match goal with
-         | [ L : Learnt _ |- _ ] => clear L
-         end.
-
-  constructor.
-  - congruence.
-  - congruence.
-  - admit. (* no_errors verilog1 *)
-  - admit. (* no_errors verilog2 *)
-  - simpl. intros.
-    unfold match_on_regs.
-    apply List.Forall_forall; intros outreg Houtreg.
-    move Hunsat at bottom.
-    unfold SMT.unsat in Hunsat.
-    move H1 at bottom.
-    destruct (H1 outreg ltac:(assumption)) as [? [ ? ? ]].
-    repeat match goal with
-           | [ H : context[match ?d with _ => _ end] |- _] =>
-               destruct d eqn:?; subst; try discriminate
-           | [ H : inr _ = inr _ |- _] => inv H
-           end.
-    destruct (regState final1 outreg) as [v|].
-    + exists v. intuition.
-        admit.
-      * admit.
-    + admit.
-Admitted.
 
 Lemma match_on_regs_trans :
   forall rs v1 v2 v3,
@@ -283,7 +173,8 @@ Lemma equivalent_trans v1 v2 v3 :
 Proof.
   intros [interface_inputs_match1 interface_outputs_match1 no_errors1 no_errors2 behaviour_match1].
   intros [interface_inputs_match2 interface_outputs_match2 _ no_errors3 behaviour_match2].
-  constructor; simpl in *.
+  unfold equivalent_behaviour in *.
+  constructor; unfold equivalent_behaviour in *; simpl in *.
   all: (try rewrite <- interface_inputs_match2 in *;
         try rewrite <- interface_inputs_match1 in *;
         try rewrite <- interface_outputs_match2 in *;
@@ -294,15 +185,16 @@ Proof.
   - congruence.
   - assumption.
   - assumption.
-  - intros.
-    specialize (behaviour_match1 input_vals ltac:(assumption) ltac:(assumption)).
-    specialize (behaviour_match2 input_vals ltac:(assumption) ltac:(assumption)).
-    assert (exists final', multistep_eval (set_regs (combine (Verilog.inputs v1) input_vals) (initial_state v2)) final') as H1. {
-      unfold no_errors in *.
-      rewrite <- interface_inputs_match2 in *.
-      rewrite <- interface_inputs_match1 in *.
-      simpl in *.
-      eauto.
+  - intros ? ? input_wf3 ? ? final3 Hrun1 Hrun3.
+    assert (input_valid v2 input) as input_wf2. {
+      unfold input_valid in *.
+      rewrite <- interface_inputs_match1.
+      assumption.
+    }
+    specialize (behaviour_match1 input ltac:(assumption) ltac:(assumption)).
+    specialize (behaviour_match2 input ltac:(assumption) ltac:(assumption)).
+    assert (exists final', run_multistep (initial_state v2 input) = Some final') as H1. {
+      unfold no_errors in *. eauto.
     }
     destruct H1.
     eapply match_on_regs_trans; eauto.
@@ -318,35 +210,1004 @@ Proof.
   - congruence.
   - assumption.
   - assumption.
-  - simpl in *. intros.
+  - simpl in *. unfold equivalent_behaviour. intros.
     rewrite <- interface_outputs_match1 in *.
-    rewrite <- interface_inputs_match1 in *.
     apply match_on_regs_sym.
     eauto.
 Qed.
 
-Theorem equivalence_query_correct verilog1 verilog2 query :
-  equivalence_query verilog1 verilog2 = inr query ->
-  SMT.unsat query ->
+Theorem canonicalize_correct v v' :
+  VerilogCanonicalize.canonicalize_verilog v = inr v' ->
+  equivalent v v'.
+Admitted.
+
+Theorem verilog_to_smt_correct tag start v smt :
+  VerilogToSMT.verilog_to_smt tag start v = inr smt ->
+  SMTLibFacts.smt_reflect
+    (SMT.query smt)
+    (fun ρ => valid_execution v (SMT.execution_of_valuation tag (SMT.nameMap smt) ρ)).
+Admitted.
+
+Lemma FIXME_no_errors v : no_errors v.
+Admitted.
+
+Remark FIXME_verilog_outputs_in_variables name v:
+  In name (Verilog.outputs v) ->
+  In name (variable_names (Verilog.modVariables v)).
+Admitted.
+
+Lemma verilog_to_smt_only_tag t n v s :
+  VerilogToSMT.verilog_to_smt t n v = inr s ->
+  VerilogSMTBijection.only_tag t (SMT.nameMap s).
+Admitted.
+
+(** This depends on typechecking pass (module does not write to its inputs) *)
+Lemma run_multistep_preserve_initial_values v input final :
+  input_valid v input ->
+  run_multistep (initial_state v input) = Some final ->
+  Forall (fun n => regState final n = regState (initial_state v input) n) (Verilog.inputs v).
+Proof. Admitted.
+
+Definition smt_same_value (var : string) (m : VerilogSMTBijection.t) (ρ : SMTLib.valuation) :=
+  exists smtName1 smtName2 v,
+    m (TaggedName.VerilogLeft, var) = Some smtName1 /\
+      m (TaggedName.VerilogRight, var) = Some smtName2 /\
+      ρ smtName1 = Some v /\
+      ρ smtName2 = Some v.
+
+Definition smt_all_same_values
+  (vars : list string) (m : VerilogSMTBijection.t) (ρ : SMTLib.valuation) :=
+  Forall (fun verilogName => smt_same_value verilogName m ρ) vars.
+
+Definition smt_distinct_value (var : string) (m : VerilogSMTBijection.t) (ρ : SMTLib.valuation) :=
+  exists smtName1 smtName2 v1 v2,
+    m (TaggedName.VerilogLeft, var) = Some smtName1 /\
+      m (TaggedName.VerilogRight, var) = Some smtName2 /\
+      ρ smtName1 = Some v1 /\
+      ρ smtName2 = Some v2 /\
+      v1 <> v2.
+
+Definition smt_has_value (tag : TaggedName.Tag) (var : string) (nameMap : VerilogSMTBijection.t) (ρ : SMTLib.valuation) :=
+  exists smtName v, nameMap (tag, var) = Some smtName /\ ρ smtName = Some v.
+
+Definition smt_all_have_values
+  (tag : TaggedName.Tag) (vars : list string) (nameMap : VerilogSMTBijection.t) (ρ : SMTLib.valuation) :=
+  Forall (fun verilogName => smt_has_value tag verilogName nameMap ρ) vars.
+
+Definition smt_some_distinct_values
+  (vars : list string) (m : VerilogSMTBijection.t) (ρ : SMTLib.valuation) :=
+  Exists (fun verilogName => smt_distinct_value verilogName m ρ) vars.
+
+Lemma mk_var_same_spec : forall name m q,
+  mk_var_same name m = inr q ->
+  SMTLibFacts.smt_reflect [q] (smt_same_value name m).
+Proof.
+  intros * Hfunc.
+  funelim (mk_var_same name m); try congruence.
+  (* destruct (size1 =? size2)%N eqn:Esize; try congruence. *)
+  (* rewrite N.eqb_eq in Esize; subst. *)
+  replace q with (SMTLib.Term_Eq (SMTLib.Term_Const smt_name1) (SMTLib.Term_Const smt_name2)) by congruence.
+  unfold smt_same_value.
+  split; intros * H.
+  - inv H. inv H2.
+    destruct (ρ smt_name1) eqn:E1 ; try discriminate.
+    destruct (ρ smt_name2) eqn:E2 ; try discriminate.
+    inv H0.
+    rewrite SMTLib.value_eqb_eq in H1. subst.
+    exists smt_name1. exists smt_name2. exists v0.
+    rewrite E1. rewrite E2.
+    intuition trivial.
+  - repeat econstructor.
+    destruct H as [smt_name1' [smt_name2' [w [v [H0 [H1 H2]]]]]].
+    replace smt_name1' with smt_name1 in * by congruence.
+    replace smt_name2' with smt_name2 in * by congruence.
+    unfold SMTLib.term_satisfied_by. simpl.
+    destruct (ρ smt_name1) eqn:E1; destruct (ρ smt_name2) eqn:E2; try discriminate.
+    repeat match goal with
+           | [ v1 : SMTLib.value, v2 : SMTLib.value, H : Some ?v1 = Some ?v2 |- _ ] =>
+               inv H
+           end.
+    replace (SMTLib.value_eqb _ _) with true
+      by (symmetry; now apply SMTLib.value_eqb_eq).
+    reflexivity.
+Qed.
+
+(* TODO: Move me to smtcoqapi *)
+Lemma smtlib_and_conj : forall (q1 q2 : SMTLib.term) (P1 P2 : SMTLib.valuation -> Prop),
+    SMTLibFacts.smt_reflect [q1] P1 ->
+    SMTLibFacts.smt_reflect [q2] P2 ->
+    SMTLibFacts.smt_reflect [SMTLib.Term_And q1 q2] (fun ρ : SMTLib.valuation => P1 ρ /\ P2 ρ).
+Proof.
+  intros * H1 H2.
+  split; intros H0.
+  - unfold SMTLib.satisfied_by in H0.
+    inv H0. inv H4.
+    destruct (SMTLib.interp_term ρ q1) as [[ b1 | ? | ? ] | ] eqn:E1; try discriminate.
+    destruct (SMTLib.interp_term ρ q2) as [[ b2 | ? | ? ] | ] eqn:E2; try discriminate.
+    inv H0. apply andb_prop in H3. intuition; subst.
+    + apply H1. repeat constructor. apply E1.
+    + apply H2. repeat constructor. apply E2.
+  - destruct H0 as [HP1 HP2].
+    repeat econstructor.
+    unfold SMTLib.term_satisfied_by. simpl.
+    replace (SMTLib.interp_term ρ q1) with (Some (SMTLib.Value_Bool true)); cycle 1. {
+      apply H1 in HP1. inv HP1. symmetry. assumption.
+    }
+    replace (SMTLib.interp_term ρ q2) with (Some (SMTLib.Value_Bool true)); cycle 1. {
+      apply H2 in HP2. inv HP2. symmetry. assumption.
+    }
+    reflexivity.
+Qed.
+    
+Lemma mk_inputs_same_spec : forall inputs m q,
+  mk_inputs_same inputs m = inr q ->
+  SMTLibFacts.smt_reflect [q] (smt_all_same_values inputs m).
+Proof.
+  intros ?. induction inputs.
+  - intros. inv H. simp mk_inputs_same.
+    unfold smt_all_same_values.
+    eapply SMTLibFacts.smt_reflect_rewrite. {
+      intros. apply Forall_nil_iff.
+    }
+    repeat constructor.
+  - intros. simp mk_inputs_same in H.
+    autodestruct_eqn E.
+    unfold smt_all_same_values.
+    eapply SMTLibFacts.smt_reflect_rewrite. {
+      intros. apply Forall_cons_iff.
+    }
+    apply smtlib_and_conj.
+    + apply mk_var_same_spec. apply E.
+    + apply IHinputs. assumption.
+Qed.
+
+Definition smtlib_is_bool ρ q := exists b, SMTLib.interp_term ρ q = Some (SMTLib.Value_Bool b).
+
+(* TODO: Move me to smtcoqapi *)
+Lemma smtlib_or_disj : forall (q1 q2 : SMTLib.term) (P1 P2 : SMTLib.valuation -> Prop),
+    SMTLibFacts.smt_reflect [q1] P1 ->
+    SMTLibFacts.smt_reflect [q2] P2 ->
+    SMTLibFacts.smt_reflect
+      [SMTLib.Term_Or q1 q2]
+      (fun ρ : SMTLib.valuation => (P1 ρ /\ smtlib_is_bool ρ q2) \/ (smtlib_is_bool ρ q1 /\ P2 ρ)).
+Proof.
+  intros * H1 H2.
+  split; intros H0.
+  - unfold SMTLib.satisfied_by in H0.
+    inv H0. inv H4.
+    destruct (SMTLib.interp_term ρ q1) as [[ b1 | ? | ? ] | ] eqn:E1; try discriminate.
+    destruct (SMTLib.interp_term ρ q2) as [[ b2 | ? | ? ] | ] eqn:E2; try discriminate.
+    unfold smtlib_is_bool.
+    inv H0. apply Bool.orb_prop in H3. intuition (subst; eauto).
+    + left. intuition eauto. 
+      apply H1. repeat constructor. apply E1.
+    + right. intuition eauto.
+      apply H2. repeat constructor. apply E2.
+  - repeat econstructor.
+    unfold SMTLib.term_satisfied_by. simpl.
+    (* destruct H0 as [[HP1 [b1 Hbool1]] | [HP2 [b2 Hbool2]]]. *)
+    destruct H0 as [[HP1 [b2 Hbool2]] | [[b1 Hbool1] HP2]].
+    + replace (SMTLib.interp_term ρ q1) with (Some (SMTLib.Value_Bool true)); cycle 1. {
+        apply H1 in HP1. inv HP1. symmetry. assumption.
+      }
+      rewrite Hbool2.
+      now rewrite Bool.orb_true_l.
+    + replace (SMTLib.interp_term ρ q2) with (Some (SMTLib.Value_Bool true)); cycle 1. {
+        apply H2 in HP2. inv HP2. symmetry. assumption.
+      }
+      rewrite Hbool1.
+      now rewrite Bool.orb_true_r.
+Qed.
+
+(* TODO: Move me to smtcoqapi *)
+Lemma value_eqb_neq v1 v2 : SMTLib.value_eqb v1 v2 = false <-> v1 <> v2.
+Proof.
+  split; intros H.
+  - intros contra.
+    apply SMTLib.value_eqb_eq in contra.
+    congruence.
+  - destruct (SMTLib.value_eqb v1 v2) eqn:E; try reflexivity.
+    apply SMTLib.value_eqb_eq in E.
+    contradiction.
+Qed.
+
+Lemma mk_var_distinct_spec : forall name m q,
+  mk_var_distinct name m = inr q ->
+  SMTLibFacts.smt_reflect [q] (smt_distinct_value name m).
+Proof.
+  intros * Hfunc.
+  funelim (mk_var_distinct name m); try congruence.
+  (* destruct (size1 =? size2)%N eqn:Esize; try congruence. *)
+  (* rewrite N.eqb_eq in Esize; subst. *)
+  replace q with (SMTLib.Term_Not (SMTLib.Term_Eq
+                                     (SMTLib.Term_Const smt_name1)
+                                     (SMTLib.Term_Const smt_name2)))
+    by congruence.
+  unfold smt_distinct_value.
+  split; intros * H.
+  - inv H. inv H2.
+    destruct (ρ smt_name1) eqn:E1 ; try discriminate.
+    destruct (ρ smt_name2) eqn:E2 ; try discriminate.
+    inv H0.
+    rewrite Bool.negb_true_iff in H1.
+    rewrite value_eqb_neq in H1. subst.
+    exists smt_name1. exists smt_name2. exists v. exists v0.
+    rewrite E1. rewrite E2.
+    intuition trivial.
+  - repeat econstructor.
+    destruct H as [smt_name1' [smt_name2' [w [v [v0 [H0 [H1 [H2 H3]]]]]]]].
+    replace smt_name1' with smt_name1 in * by congruence.
+    replace smt_name2' with smt_name2 in * by congruence.
+    unfold SMTLib.term_satisfied_by. simpl.
+    destruct (ρ smt_name1) eqn:E1; destruct (ρ smt_name2) eqn:E2; try discriminate.
+    repeat match goal with
+           | [ v1 : SMTLib.value, v2 : SMTLib.value, H : Some ?v1 = Some ?v2 |- _ ] =>
+               inv H
+           end.
+    replace (SMTLib.value_eqb _ _) with false
+      by (symmetry; now apply value_eqb_neq).
+    reflexivity.
+Qed.
+
+Lemma smtlib_is_bool_or ρ t1 t2:
+  smtlib_is_bool ρ t1 /\ smtlib_is_bool ρ t2 <-> smtlib_is_bool ρ (SMTLib.Term_Or t1 t2).
+Proof.
+  split.
+  - intros * [[v1 H1] [v2 H2]].
+    unfold smtlib_is_bool.
+    simpl. rewrite H1. rewrite H2.
+    eauto.
+  - intros [v H]. simpl in H.
+    autodestruct_eqn E.
+    unfold smtlib_is_bool in *.
+    eauto.
+Qed.
+
+Lemma mk_var_distinct_is_bool var : forall m t ρ,
+    smt_has_value TaggedName.VerilogLeft var m ρ ->
+    smt_has_value TaggedName.VerilogRight var m ρ ->
+    mk_var_distinct var m = inr t ->
+    smtlib_is_bool ρ t.
+Proof.
+  intros * Hval1 Hval2 H.
+  funelim (mk_var_distinct var m); try congruence.
+  match type of Heqcall with
+  | inr ?t' = mk_var_distinct _ _  => replace t with t' in * by congruence
+  end.
+  unfold smtlib_is_bool. simpl.
+  destruct Hval1 as [smt_name1' [v1 [? Hval1]]]. replace smt_name1' with smt_name1 in * by congruence.
+  destruct Hval2 as [smt_name2' [v2 [? Hval2]]]. replace smt_name2' with smt_name2 in * by congruence.
+  rewrite Hval1. rewrite Hval2.
+  eauto.
+Qed.
+
+Lemma mk_var_distinct_has_value var : forall m tag t ρ,
+    mk_var_distinct var m = inr t ->
+    smtlib_is_bool ρ t ->
+    smt_has_value tag var m ρ.
+Proof.
+  intros * Hdistinct Hisbool.
+  funelim (mk_var_distinct var m); try congruence.
+  match type of Heqcall with
+  | inr ?t' = mk_var_distinct _ _  => replace t with t' in * by congruence
+  end.
+  unfold smtlib_is_bool in *. simpl in *.
+  unfold smt_has_value.
+  autodestruct_eqn E; try solve_by_inverts 2%nat.
+  destruct tag; intuition eauto.
+Qed.
+
+Lemma mk_outputs_distinct_is_bool outputs : forall m t ρ,
+    smt_all_have_values TaggedName.VerilogLeft outputs m ρ ->
+    smt_all_have_values TaggedName.VerilogRight outputs m ρ ->
+    mk_outputs_distinct outputs m = inr t ->
+    smtlib_is_bool ρ t.
+Proof.
+  induction outputs; intros * Hval1 Hval2 H; simp mk_outputs_distinct in *.
+  - inv H. repeat econstructor.
+  - autodestruct_eqn E.
+    inv Hval1. inv Hval2.
+    fold (smt_all_have_values TaggedName.VerilogLeft outputs m ρ) in *.
+    fold (smt_all_have_values TaggedName.VerilogRight outputs m ρ) in *.
+    apply smtlib_is_bool_or.
+    eauto using mk_var_distinct_is_bool.
+Qed.
+
+Lemma mk_outputs_distinct_have_values outputs : forall m tag t ρ,
+    mk_outputs_distinct outputs m = inr t ->
+    smtlib_is_bool ρ t ->
+    smt_all_have_values tag outputs m ρ.
+Proof.
+  induction outputs; intros * Hdistinct Hisbool.
+  - repeat econstructor.
+  - simp mk_outputs_distinct in *.
+    autodestruct_eqn E.
+    constructor; fold (smt_all_have_values tag outputs m ρ) in *.
+    + eapply mk_var_distinct_has_value. eassumption.
+      apply smtlib_is_bool_or in Hisbool. intuition auto.
+    + eapply IHoutputs. eassumption.
+      apply smtlib_is_bool_or in Hisbool. intuition auto.
+Qed.
+
+Lemma smt_distinct_value_has_value tag var m ρ :
+  smt_distinct_value var m ρ ->
+  smt_has_value tag var m ρ.
+Proof. destruct tag; firstorder. Qed.
+
+Lemma mk_outputs_distinct_spec outputs m q:
+  mk_outputs_distinct outputs m = inr q ->
+  SMTLibFacts.smt_reflect [q] (fun ρ => smt_some_distinct_values outputs m ρ
+                                     /\ smt_all_have_values TaggedName.VerilogLeft outputs m ρ
+                                     /\ smt_all_have_values TaggedName.VerilogRight outputs m ρ).
+Proof.
+  revert q m. induction outputs.
+  - intros. inv H. simp mk_outputs_distinct.
+    unfold smt_some_distinct_values.
+    eapply SMTLibFacts.smt_reflect_rewrite with (P2 := fun _ => False). {
+      intuition (try eapply Exists_nil; eauto).
+    }
+    apply SMTLibFacts.unsat_smt_reflect_false.
+    unfold SMTLib.unsatisfiable.
+    intros * contra. inv contra. inv H1.
+  - intros.
+    simp mk_outputs_distinct in H.
+    autodestruct_eqn E.
+    specialize (IHoutputs _ _ ltac:(eassumption)).
+    unfold smt_some_distinct_values.
+    unshelve (epose proof
+                (smtlib_or_disj t t0
+                   (smt_distinct_value a m)
+                   (fun ρ => smt_some_distinct_values outputs m ρ
+                          /\ smt_all_have_values TaggedName.VerilogLeft  outputs m ρ
+                          /\ smt_all_have_values TaggedName.VerilogRight outputs m ρ) _ _) as Hreflect).
+    { auto using mk_var_distinct_spec. }
+    { assumption. }
+    eapply SMTLibFacts.smt_reflect_rewrite. 2: apply Hreflect.
+    intros. simpl.
+    unfold smt_all_have_values.
+    rewrite Exists_cons.
+    rewrite 2 Forall_cons_iff.
+    fold (smt_all_have_values TaggedName.VerilogLeft  outputs m ρ) in *.
+    fold (smt_all_have_values TaggedName.VerilogRight outputs m ρ) in *.
+    fold (smt_some_distinct_values outputs m ρ) in *.
+    intuition (eauto using mk_outputs_distinct_is_bool,
+                mk_var_distinct_is_bool,
+                smt_distinct_value_has_value,
+                mk_outputs_distinct_have_values,
+                mk_var_distinct_has_value).
+Qed.
+
+Definition counterexample_valuation v1 v2 m ρ :=
+  valid_execution v1 (SMT.execution_of_valuation TaggedName.VerilogLeft m ρ)
+  /\ valid_execution v2 (SMT.execution_of_valuation TaggedName.VerilogRight m ρ)
+  /\ smt_all_same_values (Verilog.inputs v1) m ρ
+  /\ smt_some_distinct_values (Verilog.outputs v1) m ρ
+  /\ smt_all_have_values TaggedName.VerilogLeft (Verilog.outputs v1) m ρ
+  /\ smt_all_have_values TaggedName.VerilogRight (Verilog.outputs v1) m ρ.
+
+Definition execution_same_value (e1 e2 : execution) name :=
+  exists v, e1 name = Some v /\ e2 name = Some v.
+
+Definition execution_all_same_values e1 e2 names :=
+  Forall (execution_same_value e1 e2) names.
+
+Definition execution_distinct_value (e1 e2 : execution) name :=
+  exists v1 v2, e1 name = Some v1 /\ e2 name = Some v2 /\ (XBV.has_x v1 \/ XBV.has_x v2 \/ v1 <> v2).
+
+Definition execution_some_distinct_values e1 e2 names :=
+  Exists (execution_distinct_value e1 e2) names.
+
+Definition execution_has_value (e : execution) name :=
+  exists v, e name = Some v.
+
+Definition execution_all_have_values e names :=
+  Forall (execution_has_value e) names.
+
+Definition execution_not_x (e : execution) name :=
+  forall v, e name = Some v -> ~ XBV.has_x v.
+
+Definition execution_no_exes (e : execution) names :=
+  Forall (execution_not_x e) names.
+
+Definition counterexample_execution v1 e1 v2 e2 :=
+  valid_execution v1 e1
+  /\ valid_execution v2 e2
+  /\ execution_all_same_values e1 e2 (Verilog.inputs v1)
+  /\ execution_some_distinct_values e1 e2 (Verilog.outputs v1)
+  /\ execution_all_have_values e1 (Verilog.outputs v1)
+  /\ execution_all_have_values e2 (Verilog.outputs v1).
+
+Definition only_bitvectors (ρ : SMTLib.valuation) :=
+  forall n v, ρ n = Some v -> (exists w bv, v = SMTLib.Value_BitVec w bv).
+
+Remark complete_execution_outputs_have_values e v :
+  complete_execution v e ->
+  execution_all_have_values e (Verilog.outputs v).
+Proof.
+  unfold complete_execution, execution_all_have_values.
+  intros. apply Forall_forall. intros name Hname_in_outputs.
+  apply FIXME_verilog_outputs_in_variables in Hname_in_outputs.
+  firstorder.
+Qed.
+
+Remark valid_execution_outputs_have_values e v :
+  valid_execution v e ->
+  execution_all_have_values e (Verilog.outputs v).
+Proof. eauto using valid_execution_complete, complete_execution_outputs_have_values. Qed.
+
+Theorem all_same_values_execution_of_valuation names m ρ :
+  only_bitvectors ρ ->
+  smt_all_same_values names m ρ ->
+  execution_all_same_values
+    (SMT.execution_of_valuation TaggedName.VerilogLeft m ρ)
+    (SMT.execution_of_valuation TaggedName.VerilogRight m ρ)
+    names.
+Proof.
+  intro Honly_bv.
+  unfold smt_all_same_values, execution_all_same_values in *.
+  apply Forall_impl.
+  unfold smt_same_value, execution_same_value.
+  intros ? [smtName1 [smtName2 [v [? [? [? ?]]]]]].
+  edestruct Honly_bv with (n := smtName1) as [w [bv Hbv]]; try eassumption; subst v.
+  eexists. split.
+  all: eauto using SMT.execution_of_valuation_some.
+Qed.
+
+Theorem some_distinct_values_execution_of_valuation names m ρ :
+  only_bitvectors ρ ->
+  smt_some_distinct_values names m ρ ->
+  execution_some_distinct_values
+    (SMT.execution_of_valuation TaggedName.VerilogLeft m ρ)
+    (SMT.execution_of_valuation TaggedName.VerilogRight m ρ) names.
+Proof.
+  intros Honly_bv.
+  unfold smt_some_distinct_values, execution_some_distinct_values in *.
+  apply Exists_impl.
+  unfold smt_distinct_value, execution_distinct_value.
+  intros ? [smtName1 [smtName2 [v1 [v2 [H0 [H1 [H2 [H3 H4]]]]]]]].
+  edestruct Honly_bv with (n := smtName1) as [w1 [bv1 Hbv1]]; try eassumption; subst v1.
+  edestruct Honly_bv with (n := smtName2) as [w2 [bv2 Hbv2]]; try eassumption; subst v2.
+  eexists. eexists.
+  split. { eauto using SMT.execution_of_valuation_some. }
+  split. { eauto using SMT.execution_of_valuation_some. }
+  right. right.
+  intro contra; contradict H4.
+  apply XBV.from_bv_injective in contra.
+  destruct bv1; destruct bv2. inv contra. simpl in *. now subst.
+Qed.
+
+Theorem all_have_values_execution_of_valuation tag names m ρ :
+  only_bitvectors ρ ->
+  smt_all_have_values tag names m ρ ->
+  execution_all_have_values (SMT.execution_of_valuation tag m ρ) names.
+Proof.
+  intros Honly_bv.
+  unfold smt_all_have_values, execution_all_have_values in *.
+  apply Forall_impl.
+  unfold smt_has_value, execution_has_value.
+  intros ? [smtName [v [H0 H1]]].
+  edestruct Honly_bv with (n := smtName) as [w [bv Hbv]]; try eassumption; subst v.
+  eexists.
+  eauto using SMT.execution_of_valuation_some.
+Qed.
+
+Theorem counterexample_valuation_execution v1 v2 m ρ:
+  only_bitvectors ρ ->
+  counterexample_valuation v1 v2 m ρ ->
+  counterexample_execution
+    v1 (SMT.execution_of_valuation TaggedName.VerilogLeft m ρ)
+    v2 (SMT.execution_of_valuation TaggedName.VerilogRight m ρ).
+Proof.
+  unfold counterexample_valuation, counterexample_execution.
+  intros Honly_bv [Hvalid1 [Hvalid2 [Hinputsame [Houtdistinct [Houtputsexist1 Houtputsexist2]]]]].
+  split. { assumption. }
+  split. { assumption. }
+  split. { now eapply all_same_values_execution_of_valuation. }
+  split. { now eapply some_distinct_values_execution_of_valuation. }
+  split. { now eapply all_have_values_execution_of_valuation. }
+  now eapply all_have_values_execution_of_valuation.
+Qed.
+
+Definition match_map_execution (tag : TaggedName.Tag) (m : VerilogSMTBijection.t) (e : execution) :=
+  forall name, (exists smtName, m (tag, name) = Some smtName) <-> (exists xbv, e name = Some xbv).
+
+Lemma match_map_execution_of_verilog v tag m e :
+  valid_execution v e ->
+  SMT.match_map_verilog tag m v ->
+  match_map_execution tag m e.
+Proof.
+  intros Hvalid Hmatch verilogName.
+  assert (complete_execution v e) as Hcomplete by eauto using valid_execution_complete; clear Hvalid.
+  unfold complete_execution, SMT.match_map_verilog, match_map_execution in *.
+  specialize (Hcomplete verilogName). specialize (Hmatch verilogName).
+  rewrite Hmatch. clear Hmatch.
+  firstorder.
+Qed.
+
+Lemma Forall_impl_In {A} (P Q : A -> Prop) (l : list A) :
+  (forall a : A, In a l -> P a -> Q a) ->
+  Forall P l -> Forall Q l.
+Proof. rewrite ! Forall_forall. firstorder. Qed.
+
+Lemma Exists_impl_In {A} (P Q : A -> Prop) (l : list A) :
+  (forall a : A, In a l -> P a -> Q a) ->
+  Exists P l -> Exists Q l.
+Proof.
+  rewrite ! Exists_exists.
+  intros Himpl [x [Hin HP]].
+  eauto.
+Qed.
+
+Lemma all_same_values_valuation_of_executions e1 e2 names m :
+  match_map_execution TaggedName.VerilogLeft m e1 ->
+  match_map_execution TaggedName.VerilogRight m e2 ->
+  execution_no_exes e1 names ->
+  execution_all_same_values e1 e2 names ->
+  smt_all_same_values names m (SMT.valuation_of_executions m e1 e2).
+Proof.
+  unfold smt_all_same_values, execution_all_same_values in *.
+  intros Hmatch1 Hmatch2 Hno_exes.
+  unfold execution_no_exes, execution_not_x in Hno_exes; rewrite Forall_forall in Hno_exes.
+  apply Forall_impl_In.
+  unfold smt_same_value, execution_same_value, execution_no_exes in *.
+  intros name Hname_in [bv [H1 H2]].
+  destruct Hmatch1 with (name := name) as [Hmatch1_fw Hmatch1_bw].
+  edestruct Hmatch1_bw as [smtName1 HsmtName1]. { eauto. }
+  destruct Hmatch2 with (name := name) as [Hmatch2_fw Hmatch2_bw].
+  edestruct Hmatch2_bw as [smtName2 HsmtName2]. { eauto. }
+  unfold match_map_execution in *.
+  exists smtName1. exists smtName2.
+  assert (exists v : BV.t, XBV.to_bv bv = Some v) as Hto_bv. {
+    apply XBV.not_has_x_to_bv. eauto.
+  } destruct Hto_bv.
+  erewrite SMT.valuation_of_executions_some_left; eauto.
+  erewrite SMT.valuation_of_executions_some_right; eauto.
+Qed.
+
+Lemma FIXME_valid_executions_no_exes v e name xbv :
+  valid_execution v e ->
+  e name = Some xbv ->
+  ~ XBV.has_x xbv.
+Admitted.
+
+Lemma some_distinct_values_valuation_of_executions e1 e2 names m :
+  match_map_execution TaggedName.VerilogLeft m e1 ->
+  match_map_execution TaggedName.VerilogRight m e2 ->
+  execution_no_exes e1 names ->
+  execution_no_exes e2 names ->
+  execution_some_distinct_values e1 e2 names ->
+  smt_some_distinct_values names m (SMT.valuation_of_executions m e1 e2).
+Proof.
+  unfold smt_some_distinct_values, execution_some_distinct_values in *.
+  intros Hmatch1 Hmatch2 Hno_exes1 Hno_exes2.
+  unfold execution_no_exes, execution_not_x in *; rewrite Forall_forall in Hno_exes1, Hno_exes2.
+  apply Exists_impl_In.
+  unfold smt_distinct_value, execution_distinct_value.
+  intros name Hname_in [v1 [v2 [H1 [H2 Hdistinct]]]].
+  decompose [or] Hdistinct; clear Hdistinct; try solve [exfalso; firstorder].
+  destruct Hmatch1 with (name := name) as [Hmatch1_fw Hmatch1_bw].
+  edestruct Hmatch1_bw as [smtName1 HsmtName1]. { eauto. }
+  destruct Hmatch2 with (name := name) as [Hmatch2_fw Hmatch2_bw].
+  edestruct Hmatch2_bw as [smtName2 HsmtName2]. { eauto. }
+  unfold match_map_execution in *.
+  exists smtName1. exists smtName2.
+  assert (exists bv : BV.t, XBV.to_bv v1 = Some bv) as Hto_bv1. {
+    apply XBV.not_has_x_to_bv. eauto.
+  } destruct Hto_bv1 as [bv1 Hbv1].
+  assert (exists bv : BV.t, XBV.to_bv v2 = Some bv) as Hto_bv2. {
+    apply XBV.not_has_x_to_bv. eauto.
+  } destruct Hto_bv2 as [bv2 Hbv2].
+  erewrite SMT.valuation_of_executions_some_left; eauto.
+  erewrite SMT.valuation_of_executions_some_right; eauto.
+  eexists. eexists. repeat (split; eauto).
+  intro contra. apply H0.
+  inv contra.
+  unfold BVList.RAWBITVECTOR_LIST.of_bits in *.
+  subst bv2.
+  eapply XBV.to_bv_injective; eassumption.
+Qed.
+
+Lemma all_have_values_left_valuation_of_executions e1 e2 names m :
+  execution_no_exes e1 names ->
+  match_map_execution TaggedName.VerilogLeft m e1 ->
+  execution_all_have_values e1 names ->
+  smt_all_have_values TaggedName.VerilogLeft names m (SMT.valuation_of_executions m e1 e2).
+Proof.
+  intros Hno_exes Hmatch.
+  unfold execution_all_have_values, execution_has_value, smt_all_have_values, smt_has_value, match_map_execution in *.
+  unfold execution_no_exes, execution_not_x in *; rewrite Forall_forall in Hno_exes.
+  eapply Forall_impl_In.
+  intros name Hname_in [xbv Hxbv].
+  destruct Hmatch with (name := name) as [_ [smtName HsmtName]]; eauto.
+  exists smtName.
+  assert (exists bv : BV.t, XBV.to_bv xbv = Some bv) as Hto_bv. {
+    apply XBV.not_has_x_to_bv. eauto.
+  } destruct Hto_bv as [bv Hbv].
+  erewrite SMT.valuation_of_executions_some_left; eauto.
+Qed.
+
+Lemma all_have_values_right_valuation_of_executions e1 e2 names m :
+  execution_no_exes e2 names ->
+  match_map_execution TaggedName.VerilogRight m e2 ->
+  execution_all_have_values e2 names ->
+  smt_all_have_values TaggedName.VerilogRight names m (SMT.valuation_of_executions m e1 e2).
+Proof.
+  intros Hno_exes Hmatch.
+  unfold execution_all_have_values, execution_has_value, smt_all_have_values, smt_has_value, match_map_execution in *.
+  unfold execution_no_exes, execution_not_x in *; rewrite Forall_forall in Hno_exes.
+  eapply Forall_impl_In.
+  intros name Hname_in [xbv Hxbv].
+  destruct Hmatch with (name := name) as [_ [smtName HsmtName]]; eauto.
+  exists smtName.
+  assert (exists bv : BV.t, XBV.to_bv xbv = Some bv) as Hto_bv. {
+    apply XBV.not_has_x_to_bv. eauto.
+  } destruct Hto_bv as [bv Hbv].
+  erewrite SMT.valuation_of_executions_some_right; eauto.
+Qed.
+
+Lemma counterexample_execution_valuation v1 v2 m e1 e2 :
+  SMT.match_map_verilog TaggedName.VerilogLeft m v1 ->
+  SMT.match_map_verilog TaggedName.VerilogRight m v2 ->
+  counterexample_execution v1 e1 v2 e2 ->
+  counterexample_valuation v1 v2 m (SMT.valuation_of_executions m e1 e2).
+Proof.
+  unfold counterexample_valuation, counterexample_execution.
+  intros Hmatch1 Hmatch2 [Hvalid1 [Hvalid2 [Hinputsame [Houtputdifferent [Houtputexist1 Houtputexist2]]]]].
+  assert (match_map_execution TaggedName.VerilogLeft m e1) by eauto using match_map_execution_of_verilog.
+  assert (match_map_execution TaggedName.VerilogRight m e2) by eauto using match_map_execution_of_verilog.
+  assert (forall names, execution_no_exes e1 names). {
+    intros. unfold execution_no_exes, execution_not_x. apply Forall_forall.
+    intros. eauto using FIXME_valid_executions_no_exes.
+  }
+  assert (forall names, execution_no_exes e2 names). {
+    intros. unfold execution_no_exes, execution_not_x. apply Forall_forall.
+    intros. eauto using FIXME_valid_executions_no_exes.
+  }
+  repeat split.
+  - erewrite SMT.execution_left_of_valuation_of_executions.
+    + assumption.
+    + eauto using FIXME_valid_executions_no_exes.
+    + eauto using FIXME_valid_executions_no_exes.
+    + eassumption.
+    + eauto using valid_execution_complete.
+  - erewrite SMT.execution_right_of_valuation_of_executions.
+    + assumption.
+    + eauto using FIXME_valid_executions_no_exes.
+    + eauto using FIXME_valid_executions_no_exes.
+    + eassumption.
+    + eauto using valid_execution_complete.
+  - apply all_same_values_valuation_of_executions; eauto.
+  - apply some_distinct_values_valuation_of_executions; eauto.
+  - apply all_have_values_left_valuation_of_executions; eauto.
+  - apply all_have_values_right_valuation_of_executions; eauto.
+Qed.
+
+Lemma execution_of_valuation_map_equal (m1 m2 : VerilogSMTBijection.t) tag ρ:
+  (forall n, m1 (tag, n) = m2 (tag, n)) ->
+  SMT.execution_of_valuation tag m1 ρ = SMT.execution_of_valuation tag m2 ρ.
+Proof.
+  intros.
+  unfold SMT.execution_of_valuation.
+  apply functional_extensionality.
+  intros name.
+  rewrite <- H.
+  reflexivity.
+Qed.
+
+Theorem equivalence_query_canonical_spec verilog1 verilog2 smt :
+  equivalence_query_canonical verilog1 verilog2 = inr smt ->
+  SMTLibFacts.smt_reflect
+    (SMT.query smt)
+    (counterexample_valuation verilog1 verilog2 (SMT.nameMap smt)).
+Proof.
+  unfold equivalence_query_canonical.
+  intros H.
+  inv H. autodestruct_eqn E. simpl.
+  remember (VerilogSMTBijection.combine _ _ _ _) as m_combined.
+  apply SMTLibFacts.concat_conj. {
+    eapply SMTLibFacts.smt_reflect_rewrite with
+      (P2 := (fun ρ => valid_execution verilog1 (SMT.execution_of_valuation TaggedName.VerilogLeft (SMT.nameMap s) ρ))).
+    - intros.
+      rewrite (execution_of_valuation_map_equal m_combined (SMT.nameMap s)). reflexivity.
+      replace m_combined.
+      eapply VerilogSMTBijection.combine_different_tag_left with (t2 := TaggedName.VerilogRight).
+      + discriminate.
+      + eapply verilog_to_smt_only_tag; eassumption.
+      + eapply verilog_to_smt_only_tag; eassumption.
+    - eapply verilog_to_smt_correct; eassumption.
+  }
+  apply SMTLibFacts.concat_conj. {
+    eapply SMTLibFacts.smt_reflect_rewrite with
+      (P2 := (fun ρ => valid_execution verilog2 (SMT.execution_of_valuation TaggedName.VerilogRight (SMT.nameMap s0) ρ))).
+    - intros.
+      rewrite (execution_of_valuation_map_equal m_combined (SMT.nameMap s0)). reflexivity.
+      replace m_combined.
+      eapply VerilogSMTBijection.combine_different_tag_right with (t1 := TaggedName.VerilogLeft).
+      + discriminate.
+      + eapply verilog_to_smt_only_tag; eassumption.
+      + eapply verilog_to_smt_only_tag; eassumption.
+    - eapply verilog_to_smt_correct; eassumption.
+  }
+  fold ([t] ++ [t0])%list.
+  apply SMTLibFacts.concat_conj.
+  - eapply mk_inputs_same_spec. eassumption.
+  - apply (mk_outputs_distinct_spec _ _ _ ltac:(eassumption)).
+Qed.
+
+Lemma not_distinct_same_value var m ρ :
+  smt_has_value TaggedName.VerilogLeft var m ρ ->
+  smt_has_value TaggedName.VerilogRight var m ρ ->
+  ~ (smt_distinct_value var m ρ) ->
+  smt_same_value var m ρ.
+Proof.
+  unfold smt_has_value, smt_distinct_value, smt_same_value.
+  intros [smtName1 [v1 [Hname1 Hval1]]] [smtName2 [v2 [Hname2 Hval2]]] H.
+  exists smtName1. exists smtName2. exists v1.
+  enough (v1 = v2) by intuition congruence.
+  destruct (SMTLib.value_eqb v1 v2) eqn:E.
+  - now apply SMTLib.value_eqb_eq.
+  - apply value_eqb_neq in E.
+    contradict H.
+    repeat eexists; intuition eauto.
+Qed.
+
+Lemma not_some_distinct_all_same vars m ρ :
+  smt_all_have_values TaggedName.VerilogLeft  vars m ρ ->
+  smt_all_have_values TaggedName.VerilogRight vars m ρ ->
+  ~ (smt_some_distinct_values vars m ρ) ->
+  smt_all_same_values vars m ρ.
+Proof.
+  unfold smt_some_distinct_values, smt_all_same_values, smt_all_have_values.
+  rewrite ! Forall_forall, Exists_exists.
+  intros.
+  eauto 15 using not_distinct_same_value.
+Qed.
+
+Ltac dec_left_tac :=
+  left; solve [repeat (progress eexists); firstorder].
+
+Ltac dec_right_tac :=
+  right; intros H; decompose [and] H; firstorder; solve_by_inverts 3%nat.
+
+Ltac dec_tac := solve [dec_left_tac || dec_right_tac].
+
+Instance dec_match_on_regs regs s1 s2 : DecProp (match_on_regs regs s1 s2).
+Proof.
+  unfold match_on_regs.
+  eapply @dec_Forall.
+  intros.
+  destruct (s1 x), (s2 x); try dec_tac.
+  destruct (dec (t0 = t)), (dec (XBV.has_x t)); subst;
+    dec_tac.
+Qed.
+
+Lemma run_multistep_execution v input final :
+  input_valid v input ->
+  run_multistep (initial_state v input) = Some final ->
+  valid_execution v (regState final).
+Proof. unfold valid_execution. eauto. Qed.
+
+Lemma initial_state_same_inputs v1 v2 input :
+  Verilog.inputs v1 = Verilog.inputs v2 ->
+  regState (initial_state v1 input) = regState (initial_state v2 input).
+Proof.
+  intros.
+  unfold initial_state.
+  replace (Verilog.inputs v2).
+  simpl.
+  reflexivity.
+Qed.
+
+Lemma initial_state_has_input_values v input :
+  input_valid v input ->
+  Forall (fun n => exists val, regState (initial_state v input) n = Some val) (Verilog.inputs v).
+Proof.
+  unfold input_valid, initial_state in *; simpl in *.
+  revert input.
+  induction (Verilog.inputs v). solve [auto].
+  simpl.
+  intros. destruct input as [ | input_hd input_tl ]; try discriminate.
+  simpl in H. inv H. specialize (IHl input_tl ltac:(assumption)).
+  constructor.
+  - simpl. unfold StrFunMap.insert.
+    rewrite eqb_refl. eauto.
+  - simpl. unfold StrFunMap.insert.
+    rewrite Forall_forall in *.
+    intros name Hname_in.
+    destruct (a =? name)%string; eauto.
+Qed.
+
+Lemma same_input_values_preserved v1 v2 input final1 final2
+  (inputs_same : Verilog.inputs v1 = Verilog.inputs v2)
+  (input_wf1 : input_valid v1 input)
+  (input_wf2 : input_valid v2 input)
+  (input_vals_defined : Forall (fun bv : XBV.t => ~ XBV.has_x bv) input)
+  (run1 : run_multistep (initial_state v1 input) = Some final1)
+  (run2 : run_multistep (initial_state v2 input) = Some final2) :
+  execution_all_same_values (regState final1) (regState final2) (Verilog.inputs v1).
+Proof.
+  unfold execution_all_same_values.
+  apply run_multistep_preserve_initial_values in run1; try assumption.
+  apply run_multistep_preserve_initial_values in run2; try assumption.
+  unfold execution_same_value.
+  apply Forall_forall. rewrite Forall_forall in run1, run2.
+  intros name Hname_in.
+  specialize (run1 name Hname_in).
+  rewrite <- inputs_same in run2. specialize (run2 name Hname_in).
+  rewrite run1.
+  erewrite <- initial_state_same_inputs in run2 by eassumption. rewrite run2.
+  pose proof (initial_state_has_input_values v1 input ltac:(auto)) as Hhas_values.
+  rewrite Forall_forall in Hhas_values.
+  edestruct Hhas_values; eauto.
+Qed.
+
+Instance dec_execution_distinct_value e1 e2 name :
+  DecProp (execution_distinct_value e1 e2 name).
+Proof.
+  unfold DecProp, execution_distinct_value.
+  destruct (e1 name) as [v1|] eqn:E1, (e2 name) as [v2|] eqn:E2; try dec_tac.
+  destruct (dec (v1 = v2)); try dec_tac.
+  subst v2.
+  destruct (dec (XBV.has_x v1)); dec_tac.
+Qed.
+
+Instance dec_execution_some_distinct_values e1 e2 names :
+  DecProp (execution_some_distinct_values e1 e2 names).
+Proof.
+  unfold execution_some_distinct_values.
+  typeclasses eauto.
+Qed.
+
+Lemma not_exists_forall {A} (P : A -> Prop) : (~ exists x, P x) -> forall x, ~ P x.
+Proof. firstorder. Qed.
+
+Lemma not_exists_forall2 {A B} (P : A -> B -> Prop) : (~ exists x y, P x y) -> forall x y, ~ P x y.
+Proof. firstorder. Qed.
+
+Lemma not_match_on_regs_distinct_values names st1 st2 :
+  execution_all_have_values st1 names ->
+  execution_all_have_values st2 names ->
+  ~ match_on_regs names st1 st2 ->
+  execution_some_distinct_values st1 st2 names.
+Proof.
+  unfold match_on_regs.
+  rewrite Forall_forall.
+  intros Hhave1 Hhave2 H.
+  destruct (dec (execution_some_distinct_values st1 st2 names)); try assumption.
+  contradict H.
+  intros name Hname_in.
+
+  unfold execution_some_distinct_values in n.
+
+  rewrite Exists_exists in n. eapply not_exists_forall with (x := name) in n.
+  destruct (dec (execution_distinct_value st1 st2 name));
+    try solve [firstorder]; clear n.
+  unfold execution_distinct_value in *.
+
+  unfold execution_all_have_values, execution_has_value in *.
+  rewrite Forall_forall in *.
+  edestruct Hhave1 as [v1 Hv1]; eauto. rewrite Hv1.
+  edestruct Hhave2 as [v2 Hv2]; eauto. rewrite Hv2.
+
+  eapply not_exists_forall2 with (x := v1) (y := v2) in n0.
+  destruct (dec (v1 = v2)); try solve [firstorder].
+  subst.
+
+  exists v2. repeat split.
+  destruct (dec (XBV.has_x v2)); firstorder.
+Qed.
+
+Lemma no_counterexample_equivalent v1 v2 :
+  Verilog.inputs v1 = Verilog.inputs v2 ->
+  Verilog.outputs v1 = Verilog.outputs v2 ->
+  (forall e1 e2, ~ counterexample_execution v1 e1 v2 e2) ->
+  equivalent_behaviour v1 v2.
+Proof.
+  unfold equivalent_behaviour.
+  unfold counterexample_execution.
+  intros.
+  (* unfold SMT.valid_execution in *. *)
+  reductio_ad_absurdum.
+  specialize (H1 (regState final1) (regState final2)).
+  contradict H1. repeat split.
+  - unfold valid_execution. eauto.
+  - unfold valid_execution. eauto.
+  - eapply same_input_values_preserved; eauto.
+  - eapply not_match_on_regs_distinct_values; eauto.
+    + eapply valid_execution_outputs_have_values. unfold valid_execution. eauto.
+    + replace (Verilog.outputs v1).
+      eapply valid_execution_outputs_have_values. unfold valid_execution. eauto.
+  - apply valid_execution_outputs_have_values.
+    eapply run_multistep_execution; eauto.
+  - replace (Verilog.outputs v1).
+    apply valid_execution_outputs_have_values.
+    eapply run_multistep_execution; eauto.
+Qed.
+
+Lemma equivalence_query_canonical_same_inputs v1 v2 query :
+  equivalence_query_canonical v1 v2 = inr query ->
+  Verilog.inputs v1 = Verilog.inputs v2.
+Proof.
+  intros H.
+  unfold equivalence_query_canonical in *.
+  inv H. autodestruct_eqn E. auto.
+Qed.
+
+Lemma equivalence_query_canonical_same_outputs v1 v2 query :
+  equivalence_query_canonical v1 v2 = inr query ->
+  Verilog.outputs v1 = Verilog.outputs v2.
+Proof.
+  intros H.
+  unfold equivalence_query_canonical in *.
+  inv H. autodestruct_eqn E. auto.
+Qed.
+
+Lemma match_map_verilog_tag_equal tag v (m1 m2 : VerilogSMTBijection.t) :
+  (forall n, m1 (tag, n) = m2 (tag, n)) ->
+  SMT.match_map_verilog tag m1 v ->
+  SMT.match_map_verilog tag m2 v.
+Proof.
+  unfold SMT.match_map_verilog.
+  intros Heq Hmatch.
+  intros verilogName. specialize (Hmatch verilogName).
+  now rewrite Heq in Hmatch.
+Qed.
+
+Theorem equivalence_query_canonical_correct verilog1 verilog2 query :
+  equivalence_query_canonical verilog1 verilog2 = inr query ->
+  SMTLib.unsatisfiable (SMT.query query) ->
   equivalent verilog1 verilog2.
 Proof.
   intros Hquery Hunsat.
-  unfold equivalence_query in *.
-  inv Hquery.
-  repeat
-    match goal with
-    | [ H : (match ?m with _ => _ end) = _ |- _ ] =>
-        destruct m eqn:?; try discriminate
-    end.
-  repeat match goal with
-         | [ H : VerilogCanonicalize.canonicalize_verilog _ = inr _ |- _ ] =>
-             apply canonicalize_correct in H
-         end.
-  repeat match goal with
-         | [ H : VerilogToSMT.verilog_to_smt _ _ = inr _ |- _ ] =>
-             pose proof (verilog_to_smt_correct _ _ _ H); clear H
-         end.
-  intuition eauto using equivalent_trans, equivalent_sym, equivalence_query_canonical_correct.
+  pose proof (equivalence_query_canonical_spec _ _ _ Hquery).
+  assert (forall e1 e2, not (counterexample_valuation verilog1 verilog2 (SMT.nameMap query)
+                      (SMT.valuation_of_executions (SMT.nameMap query) e1 e2))). {
+    intros.
+    eapply SMTLibFacts.unsat_negation; eassumption.
+  }
+  clear Hunsat. clear H.
+  constructor.
+  - unfold equivalence_query_canonical in *.
+    inv Hquery. autodestruct_eqn E. auto.
+  - unfold equivalence_query_canonical in *.
+    inv Hquery. autodestruct_eqn E. auto.
+  - apply FIXME_no_errors.
+  - apply FIXME_no_errors.
+  - eapply no_counterexample_equivalent.
+    + eauto using equivalence_query_canonical_same_inputs.
+    + eauto using equivalence_query_canonical_same_outputs.
+    + intros * contra.
+      specialize (H0 e1 e2). eapply H0. clear H0.
+      eapply counterexample_execution_valuation.
+      * unfold equivalence_query_canonical in Hquery; inv Hquery; autodestruct_eqn E.
+        simpl.
+        eapply match_map_verilog_tag_equal with (m1 := (SMT.nameMap s)).
+        -- intros.
+           erewrite VerilogSMTBijection.combine_different_tag_left with (t2 := TaggedName.VerilogRight);
+             try discriminate; eauto using verilog_to_smt_only_tag.
+        -- eapply VerilogToSMT.verilog_to_smt_map_match; eauto.
+      * unfold equivalence_query_canonical in Hquery; inv Hquery; autodestruct_eqn E.
+        simpl.
+        eapply match_map_verilog_tag_equal with (m1 := (SMT.nameMap s0)).
+        -- intros.
+           erewrite VerilogSMTBijection.combine_different_tag_right with (t1 := TaggedName.VerilogLeft);
+             try discriminate; eauto using verilog_to_smt_only_tag.
+        -- eapply VerilogToSMT.verilog_to_smt_map_match; eauto.
+      * eassumption.
+Qed.
+
+Theorem equivalence_query_correct verilog1 verilog2 query :
+  equivalence_query verilog1 verilog2 = inr query ->
+  SMTLib.unsatisfiable (SMT.query query) ->
+  equivalent verilog1 verilog2.
+Proof.
+  intros Hquery Hunsat.
+  unfold equivalence_query in *; inv Hquery; autodestruct_eqn E.
+  eauto 10 using
+    equivalent_trans,
+    equivalent_sym,
+    canonicalize_correct,
+    equivalence_query_canonical_correct.
 Qed.
 
 Print Assumptions equivalence_query_correct.
