vera/Decidable.v
@@ -1,0 +1,106 @@
+From Coq Require Import List.
+From Coq Require Import String.
+From Coq Require Import BinNums.
+From Coq Require Import BinNat.
+From Coq Require Import BinInt.
+From Coq Require Import PeanoNat.
+
+Class DecProp (P : Prop) := dec : { P } + { ~ P } .
+
+Arguments dec _ {_}.
+
+Notation mk_dec_eq :=
+  ltac:(unfold DecProp in *; repeat (decide equality || eauto))
+         (only parsing).
+
+Notation "mk_dec_eq!( x )" :=
+  ltac:(unfold DecProp in *; eauto using x; repeat (decide equality || eauto))
+         (only parsing).
+
+Notation "mk_dec_eq( x )" :=
+  ltac:(unfold DecProp in *; eauto using x)
+         (only parsing).
+
+Instance dec_not {P} `{DecProp P} : DecProp (~ P ).
+Proof. firstorder. Qed.
+
+Instance dec_and {P Q} `{DecProp P, DecProp Q} : DecProp ( P /\ Q ).
+Proof. firstorder. Qed.
+
+Instance dec_or {P Q} `{DecProp P, DecProp Q} : DecProp ( P \/ Q ).
+Proof. firstorder. Qed.
+
+Instance dec_impl {P Q} `{DecProp P, DecProp Q} : DecProp ( P -> Q ).
+Proof. firstorder. Qed.
+
+Instance dec_iff {P Q} `{DecProp P, DecProp Q} : DecProp ( P <-> Q ).
+Proof. firstorder. Qed.
+
+Instance dec_eq_string (x y : string) : DecProp (x = y) :=
+  mk_dec_eq(String.string_dec).
+
+Instance dec_eq_nat (x y : nat) : DecProp (x = y) :=
+  mk_dec_eq(Nat.eq_dec).
+
+Instance dec_eq_N (x y : N) : DecProp (x = y) :=
+  mk_dec_eq(N.eq_dec).
+
+Instance dec_eq_Z (x y : Z) : DecProp (x = y) :=
+  mk_dec_eq(Z.eq_dec).
+
+Instance dec_eq_opt {A} `{forall (x y : A), DecProp (x = y)} (x y : option A) : DecProp (x = y) :=
+  mk_dec_eq.
+
+Instance dec_eq_pair {A B}
+  `{forall (x y : A), DecProp (x = y)}
+  `{forall (x y : B), DecProp (x = y)}
+  (x y : (A * B)) : DecProp (x = y) :=
+  mk_dec_eq.
+
+Instance dec_eq_list {A} `{forall (x y : A), DecProp (x = y)} (x y : list A) : DecProp (x = y) :=
+  mk_dec_eq!(list_eq_dec).
+
+Instance dec_Forall {A} {P : A -> Prop} {decP : forall x, DecProp (P x)} l :
+  DecProp (Forall P l).
+Proof.
+  induction l.
+  - left. constructor.
+  - destruct IHl.
+    + destruct (dec (P a)).
+      * left. constructor; assumption.
+      * right. inversion 1. contradiction.
+    + right. inversion 1. contradiction.
+Qed.
+
+Instance dec_Exists {A} {P : A -> Prop} {decP : forall x, DecProp (P x)} l :
+  DecProp (Exists P l).
+Proof.
+  intros.
+  induction l.
+  - right. inversion 1.
+  - destruct (decP a).
+    + left. auto.
+    + destruct IHl.
+      * left. auto.
+      * right. inversion 1; subst; contradiction.
+Qed.
+
+Instance dec_NoDup {A}
+  `{a_dec : forall (x y: A), DecProp (x = y)}
+  (l : list A) :
+  DecProp ( List.NoDup l ).
+Proof.
+  induction l.
+  - repeat constructor.
+  - destruct IHl as [ IHl | IHl ].
+    + edestruct (List.in_dec a_dec a l).
+      * right. inversion 1. contradiction.
+      * left. constructor; assumption.
+    + right. inversion 1. contradiction.
+Qed.
+
+Definition assert_dec {E} (P : Prop) `{ DecProp P } (err : E) : sum E P :=
+  match dec P with
+  | right _ => inl err
+  | left prf => inr prf
+  end.
