vera/Tactics.v
@@ -1,3 +1,19 @@
+From Coq Require Export Lia.
+
+From vera Require Import Decidable.
+
+(* Stuff every "finisher" tactic you can think of in here *)
+Ltac crush :=
+  solve [repeat progress (
+             discriminate
+             || lia
+             || congruence
+             || auto
+             || eauto
+             || firstorder
+    )].
+
+
 (* This tactic due to Clement Pit-Claudel with some minor additions by JDP to
    allow the result to be named: https://pit-claudel.fr/clement/MSc/#org96a1b5f *)
 Inductive Learnt {A: Type} (a: A) :=
@@ -25,10 +41,41 @@ Ltac solve_by_inverts n :=
   match goal with | H : ?T |- _ =>
     match type of T with Prop =>
       inversion H;
-      match n with S (S (?n')) => subst; try constructor; solve_by_inverts (S n') end
+      match n with S (S (?n')) => subst; try constructor; try contradiction; try discriminate; solve_by_inverts (S n') end
     end
   end.
 
 Ltac solve_by_invert := solve_by_inverts 1.
 
 Ltac inv H := inversion H; subst; clear H.
+
+Ltac autodestruct :=
+  repeat match goal with
+    | [ H : context [ match ?x with _ => _ end ] |- _ ] =>
+        destruct x; try discriminate
+    | [ |- context [ match ?x with _ => _ end ] ] =>
+        destruct x; try discriminate
+    | [ H : inr _ = inr _ |- _ ] =>
+        inv H
+    | [ H : Some _ = Some _ |- _ ] =>
+        inv H
+    end.
+
+Ltac autodestruct_eqn name :=
+  repeat match goal with
+    | [ H : context [ match ?x with _ => _ end ] |- _ ] =>
+        let E := fresh name in
+        destruct x eqn:E; try discriminate
+    | [ |- context [ match ?x with _ => _ end ] ] =>
+        let E := fresh name in
+        destruct x eqn:E; try discriminate
+    | [ H : inr _ = inr _ |- _ ] =>
+        inv H
+    | [ H : Some _ = Some _ |- _ ] =>
+        inv H
+    end.
+
+Ltac reductio_ad_absurdum :=
+  match goal with
+  | [ |- ?g ] => destruct (dec g); try assumption; exfalso
+  end.
