vera/VerilogCanonicalizeCorrect.v
@@ -10,9 +10,3 @@ Import (notations) Bitvector.BV.
 Import ListNotations.
 Local Open Scope monad_scope.
 Local Open Scope bv_scope.
-
-Theorem canonicalize_correct (m1 m2 : Verilog.vmodule) (st_final : CombinationalOnly.VerilogState) :
-  canonicalize_module m1 = inr m2 ->
-  CombinationalOnly.multistep_eval (CombinationalOnly.initial_state m1) st_final ->
-  CombinationalOnly.multistep_eval (CombinationalOnly.initial_state m2) st_final.
-Admitted.
